---
title: "305 Lecture 14 - Explosion"
author: "Brian Weatherson"
date: "July 8, 2020"
output: 
  beamer_presentation:
    md_extensions: +link_attributes
    keep_tex: true
    latex_engine: xelatex
    includes:
      in_header: 305-beamer-header.tex
---

## Plan for Today

- We're going to talk two interesting consequences of the rules we've produced so far.
- The first is that the rules validate explosion, the idea that everything follows from a contradiction.
- The second is that they validate all four of what are called DeMorgan's Laws.

## Associated Reading

No associated reading, but again, this will be relevant to our later work.

# Explosion

## What It is

$P, \neg P \vdash Q$

## One Weird Thing About it

It violates **relevance** - the constraint that any valid argument should have at least some term in common between premise and conclusion.

## Informal Argument

> - An argument is valid if it is impossible for the premises to be true and the conclusion false.
> - In **Explosion**, it is impossible for the premises to be true.
> - So in **Explosion**, it is impossible for the premises to be true and the conclusion false.
> - So **Explosion** is valid.

## Formal Argument

Prove **Explosion** in Carnap.

## First Attempt

![$P, \neg P \vdash Q$](../images/class05/Class-05-5.png)

## Second Attempt

![$P, \neg P \vdash Q$](../images/class05/Class-05-6.png)

## Choice Point

1. Reject Addition
2. Reject Disjunctive Syllogism
3. Accept Explosion

> - Most people who reject explosion also reject disjunctive syllogism.

## Why Reject Explosion

> 1. Truth in a Database
> 2. Truth in a Story
> 3. There are actual true contradictions, but some things are not true.

## My View

Explosion is fine - we just have to be careful with databases and stories.

# DeMorgan Laws

## First Equivalence

1. $\neg (P \vee Q)$
2. $\neg P \wedge \neg Q$

Prove these are equivalent.

## First Direction

![$\neg (P \vee Q) \vdash \neg P \wedge \neg Q$](../images/class05/Class-05-7.png)

## Second Direction

![$\neg P \wedge \neg Q \vdash \neg (P \vee Q)$](../images/class05/Class-05-8.png)

## Second Equivalence

1. $\neg P \vee \neg Q$
2. $\neg (P \wedge Q)$

## First Direction

![$\neg (P \wedge Q) \vdash \neg P \vee \neg Q$](../images/class05/Class-05-9.png)

## Second Direction

![$\neg (P \wedge Q) \vdash \neg P \vee \neg Q$](../images/class05/Class-05-10.png)

## General Principle

To move a negation from outside the parentheses to inside it, you do two things.

1. Negate each of the parts.
2. Flip the conjunction/disjunction symbol upside down.

This process is reversible.

## For Next Time

Do the weekly assignment, and we'll start talking about truth tables.

