---
title: "305 Lecture 58 - Examples"
author: "Brian Weatherson"
date: "August 5, 2020"
output: 
  beamer_presentation:
    md_extensions: +link_attributes
    keep_tex: true
    latex_engine: xelatex
    includes:
      in_header: 305-beamer-header.tex
---

## Plan

- Examples of how to do modal tableau

## Associated Reading

- Boxes and Diamonds, chapter 5

# $\Box \Diamond A \rightarrow \Diamond \Box B$ (in S4)

## $\Box \Diamond A \rightarrow \Diamond \Box B$

\begin{oltableau}
[\pFmla{\False}{\Box \Diamond A \rightarrow \Diamond \Box B}{1}, just = \TAss,
]
\end{oltableau}

Start by saying the sentence is false.

## $\Box \Diamond A \rightarrow \Diamond \Box B$

\begin{oltableau}
[\pFmla{\False}{\Box \Diamond A \rightarrow \Diamond \Box B}{1}, just = \TAss,
  [\pFmla{\True}{\Box \Diamond A}{1}, just = {\TRule{\False}{\rightarrow}[1]},
    [\pFmla{\False}{\Diamond \Box B}{1}, just = {\TRule{\False}{\rightarrow}[1]},
    ]
  ]
]
\end{oltableau}

It's a false conditional, so true antecedent and false consequent.

## $\Box \Diamond A \rightarrow \Diamond \Box B$

\begin{oltableau}
[\pFmla{\False}{\Box \Diamond A \rightarrow \Diamond \Box B}{1}, just = \TAss,
  [\pFmla{\True}{\Box \Diamond A}{1}, just = {\TRule{\False}{\rightarrow}[1]},
    [\pFmla{\False}{\Diamond \Box B}{1}, just = {\TRule{\False}{\rightarrow}[1]},
      [\pFmla{\True}{\Diamond A}{1}, just={T $\Box$, 2},
        [\pFmla{\False}{\Box B}{1}, just={T $\Diamond$, 2},
        ]
      ]
    ]
  ]
]
\end{oltableau}

We're in a logic with T, so apply the T rules.

## $\Box \Diamond A \rightarrow \Diamond \Box B$

\begin{oltableau}
[\pFmla{\False}{\Box \Diamond A \rightarrow \Diamond \Box B}{1}, just = \TAss,
  [\pFmla{\True}{\Box \Diamond A}{1}, just = {\TRule{\False}{\rightarrow}[1]},
    [\pFmla{\False}{\Diamond \Box B}{1}, just = {\TRule{\False}{\rightarrow}[1]},
      [\pFmla{\True}{\Diamond A}{1}, just={T $\Box$, 2},
        [\pFmla{\False}{\Box B}{1}, just={T $\Diamond$, 2},
          [\pFmla{\True}{A}{1.1}, just={\TRule{\True}{\Diamond}[4]},
          ]
        ]
      ]
    ]
  ]
]
\end{oltableau}

Now apply the rule for a true diamond sentence.

## $\Box \Diamond A \rightarrow \Diamond \Box B$

\begin{oltableau}
[\pFmla{\False}{\Box \Diamond A \rightarrow \Diamond \Box B}{1}, just = \TAss,
  [\pFmla{\True}{\Box \Diamond A}{1}, just = {\TRule{\False}{\rightarrow}[1]},
    [\pFmla{\False}{\Diamond \Box B}{1}, just = {\TRule{\False}{\rightarrow}[1]},
      [\pFmla{\True}{\Diamond A}{1}, just={T $\Box$, 2},
        [\pFmla{\False}{\Box B}{1}, just={T $\Diamond$, 2},
          [\pFmla{\True}{A}{1.1}, just={\TRule{\True}{\Diamond}[4]},
            [\pFmla{\True}{\Diamond A}{1.1}, just={\TRule{\Box}{\True}[2]},
              [\pFmla{\False}{\Box B}{1.1}, just={\TRule{\False}{\Diamond}[3]},
              ]
            ]
          ]
        ]
      ]
    ]
  ]
]
\end{oltableau}

K means that we have more work to do from 2 and 3.

## $\Box \Diamond A \rightarrow \Diamond \Box B$

\begin{oltableau}
[\pFmla{\False}{\Box \Diamond A \rightarrow \Diamond \Box B}{1}, just = \TAss,
  [\pFmla{\True}{\Box \Diamond A}{1}, just = {\TRule{\False}{\rightarrow}[1]},
    [\pFmla{\False}{\Diamond \Box B}{1}, just = {\TRule{\False}{\rightarrow}[1]},
      [\pFmla{\True}{\Diamond A}{1}, just={T $\Box$, 2},
        [\pFmla{\False}{\Box B}{1}, just={T $\Diamond$, 2},
          [\pFmla{\True}{A}{1.1}, just={\TRule{\True}{\Diamond}[4]},
            [\pFmla{\True}{\Diamond A}{1.1}, just={\TRule{\Box}{\True}[2]},
              [\pFmla{\False}{\Box B}{1.1}, just={\TRule{\False}{\Diamond}[3]},
                [\pFmla{\True}{\Box \Diamond A}{1.1}, just = {4 $\Box$, 2},
                ]
              ]
            ]
          ]
        ]
      ]
    ]
  ]
]
\end{oltableau}

And 4 means that we have to carry down line 2 as well.

## $\Box \Diamond A \rightarrow \Diamond \Box B$

\begin{oltableau}
[\pFmla{\False}{\Box \Diamond A \rightarrow \Diamond \Box B}{1}, just = \TAss,
  [\pFmla{\True}{\Box \Diamond A}{1}, just = {\TRule{\False}{\rightarrow}[1]},
    [\pFmla{\False}{\Diamond \Box B}{1}, just = {\TRule{\False}{\rightarrow}[1]},
      [\pFmla{\True}{\Diamond A}{1}, just={T $\Box$, 2},
        [\pFmla{\False}{\Box B}{1}, just={T $\Diamond$, 2},
          [\pFmla{\True}{A}{1.1}, just={\TRule{\True}{\Diamond}[4]},
            [\pFmla{\True}{\Diamond A}{1.1}, just={\TRule{\Box}{\True}[2]},
              [\pFmla{\False}{\Box B}{1.1}, just={\TRule{\False}{\Diamond}[3]},
                [\pFmla{\True}{\Box \Diamond A}{1.1}, just = {4 $\Box$, 2},
                ]
              ]
            ]
          ]
        ]
      ]
    ]
  ]
]
\end{oltableau}

And I'm not going to go on because you can hopefully see the last three lines iterate indefinitely.

# $(\Diamond A \vee \Diamond B) \rightarrow \Diamond (A \vee B)$ (in K)

## $(\Diamond A \vee \Diamond B) \rightarrow \Diamond (A \vee B)$

\begin{oltableau}
[\pFmla{\False}{(\Diamond A \vee \Diamond B) \rightarrow \Diamond (A \vee B)}{1}, just = \TAss,
]
\end{oltableau}

\bigskip

Start with it being false at 1.

## $(\Diamond A \vee \Diamond B) \rightarrow \Diamond (A \vee B)$

\begin{oltableau}
[\pFmla{\False}{(\Diamond A \vee \Diamond B) \rightarrow \Diamond (A \vee B)}{1}, just = \TAss,
  [\pFmla{\True}{\Diamond A \vee \Diamond B}{1}, just = {\TRule{\False}{\rightarrow}[1]},
    [\pFmla{\False}{\Diamond (A \vee B)}{1}, just = {\TRule{\False}{\rightarrow}[1]}
    ]
  ]
]
\end{oltableau}

\bigskip

True antecedent, false consequent.

## $(\Diamond A \vee \Diamond B) \rightarrow \Diamond (A \vee B)$

\begin{oltableau}
[\pFmla{\False}{(\Diamond A \vee \Diamond B) \rightarrow \Diamond (A \vee B)}{1}, just = \TAss,
  [\pFmla{\True}{\Diamond A \vee \Diamond B}{1}, just = {\TRule{\False}{\rightarrow}[1]},
    [\pFmla{\False}{\Diamond (A \vee B)}{1}, just = {\TRule{\False}{\rightarrow}[1]},
      [\pFmla{\True}{\Diamond A}{1}, just = {\TRule{\True}{\vee}[2]}]
      [\pFmla{\True}{\Diamond B}{1}, just = {\TRule{\True}{\vee}[2]}]
    ]
  ]
]
\end{oltableau}

\bigskip

Nothing to do but branch.


## $(\Diamond A \vee \Diamond B) \rightarrow \Diamond (A \vee B)$

\begin{oltableau}
[\pFmla{\False}{(\Diamond A \vee \Diamond B) \rightarrow \Diamond (A \vee B)}{1}, just = \TAss,
  [\pFmla{\True}{\Diamond A \vee \Diamond B}{1}, just = {\TRule{\False}{\rightarrow}[1]},
    [\pFmla{\False}{\Diamond (A \vee B)}{1}, just = {\TRule{\False}{\rightarrow}[1]},
      [\pFmla{\True}{\Diamond A}{1}, just = {\TRule{\True}{\vee}[2]}
        [\pFmla{\True}{A}{1.1}, just = {\TRule{\True}{\Diamond}[4]}
        ]
      ]
      [\pFmla{\True}{\Diamond B}{1}, just = {\TRule{\True}{\vee}[2]}
        [\pFmla{\True}{B}{1.2}, just = {\TRule{\True}{\Diamond}[4]}
        ]
      ]
    ]
  ]
]
\end{oltableau}

\bigskip

Diamond sentences have to be made true somehow.

## $(\Diamond A \vee \Diamond B) \rightarrow \Diamond (A \vee B)$

\begin{oltableau}
[\pFmla{\False}{(\Diamond A \vee \Diamond B) \rightarrow \Diamond (A \vee B)}{1}, just = \TAss,
  [\pFmla{\True}{\Diamond A \vee \Diamond B}{1}, just = {\TRule{\False}{\rightarrow}[1]},
    [\pFmla{\False}{\Diamond (A \vee B)}{1}, just = {\TRule{\False}{\rightarrow}[1]},
      [\pFmla{\True}{\Diamond A}{1}, just = {\TRule{\True}{\vee}[2]}
        [\pFmla{\True}{A}{1.1}, just = {\TRule{\True}{\Diamond}[4]}
          [\pFmla{\False}{A \vee B}{1.1},  just = {\TRule{\False}{\Diamond}[3]}
          ]
        ]
      ]
      [\pFmla{\True}{\Diamond B}{1}, just = {\TRule{\True}{\vee}[2]}
        [\pFmla{\True}{B}{1.2}, just = {\TRule{\True}{\Diamond}[4]}
          [\pFmla{\False}{A \vee B}{1.2},  just = {\TRule{\False}{\Diamond}[3]}
          ]
        ]
      ]
    ]
  ]
]
\end{oltableau}

\bigskip

False diamond sentences are false at all accessible worlds.

## $(\Diamond A \vee \Diamond B) \rightarrow \Diamond (A \vee B)$

\begin{oltableau}
[\pFmla{\False}{(\Diamond A \vee \Diamond B) \rightarrow \Diamond (A \vee B)}{1}, just = \TAss,
  [\pFmla{\True}{\Diamond A \vee \Diamond B}{1}, just = {\TRule{\False}{\rightarrow}[1]},
    [\pFmla{\False}{\Diamond (A \vee B)}{1}, just = {\TRule{\False}{\rightarrow}[1]},
      [\pFmla{\True}{\Diamond A}{1}, just = {\TRule{\True}{\vee}[2]}
        [\pFmla{\True}{A}{1.1}, just = {\TRule{\True}{\Diamond}[4]}
          [\pFmla{\False}{A \vee B}{1.1},  just = {\TRule{\False}{\Diamond}[3]}
            [\pFmla{\False}{A}{1.1}, just = {\TRule{\False}{\vee}[6]}, close]
          ]
        ]
      ]
      [\pFmla{\True}{\Diamond B}{1}, just = {\TRule{\True}{\vee}[2]}
        [\pFmla{\True}{B}{1.2}, just = {\TRule{\True}{\Diamond}[4]}
          [\pFmla{\False}{A \vee B}{1.2},  just = {\TRule{\False}{\Diamond}[3]}
            [\pFmla{\False}{B}{1.2}, just = {\TRule{\False}{\vee}[6]}, close]
          ]
        ]
      ]
    ]
  ]
]
\end{oltableau}

\bigskip

And false or sentences have each side of the or false.

## $(\Diamond A \vee \Diamond B) \rightarrow \Diamond (A \vee B)$

\begin{oltableau}
[\pFmla{\False}{(\Diamond A \vee \Diamond B) \rightarrow \Diamond (A \vee B)}{1}, just = \TAss,
  [\pFmla{\True}{\Diamond A \vee \Diamond B}{1}, just = {\TRule{\False}{\rightarrow}[1]},
    [\pFmla{\False}{\Diamond (A \vee B)}{1}, just = {\TRule{\False}{\rightarrow}[1]},
      [\pFmla{\True}{\Diamond A}{1}, just = {\TRule{\True}{\vee}[2]}
        [\pFmla{\True}{A}{1.1}, just = {\TRule{\True}{\Diamond}[4]}
          [\pFmla{\False}{A \vee B}{1.1},  just = {\TRule{\False}{\Diamond}[3]}
            [\pFmla{\False}{A}{1.1}, just = {\TRule{\False}{\vee}[6]}, close]
          ]
        ]
      ]
      [\pFmla{\True}{\Diamond B}{1}, just = {\TRule{\True}{\vee}[2]}
        [\pFmla{\True}{B}{1.2}, just = {\TRule{\True}{\Diamond}[4]}
          [\pFmla{\False}{A \vee B}{1.2},  just = {\TRule{\False}{\Diamond}[3]}
            [\pFmla{\False}{B}{1.2}, just = {\TRule{\False}{\vee}[6]}, close]
          ]
        ]
      ]
    ]
  ]
]
\end{oltableau}

I've cheated a bit here by just listing one justification for the lines after the branch. It's ok because the tree is completely symmetric; the same thing happens on each branch.

# $(\Diamond A \wedge \Diamond B) \rightarrow \Diamond (A \wedge B)$ (in K)


## Hypothesis

$(\Diamond A \wedge \Diamond B) \rightarrow \Diamond (A \wedge B)$ is a theorem of K.

- So we can use the base modal rules.

## $(\Diamond A \wedge \Diamond B) \rightarrow \Diamond (A \wedge B)$

\begin{oltableau}
[\pFmla{\False}{(\Diamond A \wedge \Diamond B) \rightarrow \Diamond (A \wedge B)}{1}, just = \TAss,
]
\end{oltableau}

\bigskip

Start with it being false at 1.

## $(\Diamond A \wedge \Diamond B) \rightarrow \Diamond (A \wedge B)$

\begin{oltableau}
[\pFmla{\False}{(\Diamond A \wedge \Diamond B) \rightarrow \Diamond (A \wedge B)}{1}, just = \TAss,
  [\pFmla{\True}{\Diamond A \wedge \Diamond B}{1}, just = {\TRule{\False}{\rightarrow}[1]},
    [\pFmla{\False}{\Diamond (A \wedge B)}{1}, just = {\TRule{\False}{\rightarrow}[1]}
    ]
  ]
]
\end{oltableau}

\bigskip

True antecedent, false consequent.

## $(\Diamond A \wedge \Diamond B) \rightarrow \Diamond (A \wedge B)$

\begin{oltableau}
[\pFmla{\False}{(\Diamond A \wedge \Diamond B) \rightarrow \Diamond (A \wedge B)}{1}, just = \TAss,
  [\pFmla{\True}{\Diamond A \wedge \Diamond B}{1}, just = {\TRule{\False}{\rightarrow}[1]},
    [\pFmla{\False}{\Diamond (A \wedge B)}{1}, just = {\TRule{\False}{\rightarrow}[1]}
      [\pFmla{\True}{\Diamond A}{1}, just = {\TRule{\True}{\wedge}[2]}
        [\pFmla{\True}{\Diamond B}{1}, just = {\TRule{\True}{\wedge}[2]}
        ]
      ]
    ]
  ]
]
\end{oltableau}

\bigskip

Break up the and.

## $(\Diamond A \wedge \Diamond B) \rightarrow \Diamond (A \wedge B)$

\begin{oltableau}
[\pFmla{\False}{(\Diamond A \wedge \Diamond B) \rightarrow \Diamond (A \wedge B)}{1}, just = \TAss,
  [\pFmla{\True}{\Diamond A \wedge \Diamond B}{1}, just = {\TRule{\False}{\rightarrow}[1]},
    [\pFmla{\False}{\Diamond (A \wedge B)}{1}, just = {\TRule{\False}{\rightarrow}[1]}
      [\pFmla{\True}{\Diamond A}{1}, just = {\TRule{\True}{\wedge}[2]}
        [\pFmla{\True}{\Diamond B}{1}, just = {\TRule{\True}{\wedge}[2]}
          [\pFmla{\True}{A}{1.1}, just = {\TRule{\True}{\Diamond}[4]}
          ]
        ]
      ]
    ]
  ]
]
\end{oltableau}

\bigskip

Make $\Diamond A$ true.

## $(\Diamond A \wedge \Diamond B) \rightarrow \Diamond (A \wedge B)$

\begin{oltableau}
[\pFmla{\False}{(\Diamond A \wedge \Diamond B) \rightarrow \Diamond (A \wedge B)}{1}, just = \TAss,
  [\pFmla{\True}{\Diamond A \wedge \Diamond B}{1}, just = {\TRule{\False}{\rightarrow}[1]},
    [\pFmla{\False}{\Diamond (A \wedge B)}{1}, just = {\TRule{\False}{\rightarrow}[1]}
      [\pFmla{\True}{\Diamond A}{1}, just = {\TRule{\True}{\wedge}[2]}
        [\pFmla{\True}{\Diamond B}{1}, just = {\TRule{\True}{\wedge}[2]}
          [\pFmla{\True}{A}{1.1}, just = {\TRule{\True}{\Diamond}[4]}
            [\pFmla{\False}{A \wedge B}{1.1}, just = {\TRule{\False}{\Diamond}[3]}
              [\pFmla{\False}{A}{1.1}, just = {\TRule{\False}{\wedge}[7]}, close]
              [\pFmla{\False}{B}{1.1}, just = {\TRule{\False}{\wedge}[7]}
              ]
            ]
          ]
        ]
      ]
    ]
  ]
]
\end{oltableau}

\bigskip

Two ways for $A \wedge B$ to fail; only one is possible.

## $(\Diamond A \wedge \Diamond B) \rightarrow \Diamond (A \wedge B)$

\begin{oltableau}
[\pFmla{\False}{(\Diamond A \wedge \Diamond B) \rightarrow \Diamond (A \wedge B)}{1}, just = \TAss,
  [\pFmla{\True}{\Diamond A \wedge \Diamond B}{1}, just = {\TRule{\False}{\rightarrow}[1]},
    [\pFmla{\False}{\Diamond (A \wedge B)}{1}, just = {\TRule{\False}{\rightarrow}[1]}
      [\pFmla{\True}{\Diamond A}{1}, just = {\TRule{\True}{\wedge}[2]}
        [\pFmla{\True}{\Diamond B}{1}, just = {\TRule{\True}{\wedge}[2]}
          [\pFmla{\True}{A}{1.1}, just = {\TRule{\True}{\Diamond}[4]}
            [\pFmla{\False}{A \wedge B}{1.1}, just = {\TRule{\False}{\Diamond}[3]}
              [\pFmla{\False}{A}{1.1}, just = {\TRule{\False}{\wedge}[7]}, close]
              [\pFmla{\False}{B}{1.1}, just = {\TRule{\False}{\wedge}[7]}
                  [\pFmla{\True}{B}{1.2}, just = {\TRule{\True}{\Diamond}[5]}
                    [\pFmla{\False}{A \wedge B}{1.2}, just = {\TRule{\False}{\Diamond}[3]}
                    ]
                  ]
              ]
            ]
          ]
        ]
      ]
    ]
  ]
]
\end{oltableau}

$A \wedge B$ is still impossible.

## $(\Diamond A \wedge \Diamond B) \rightarrow \Diamond (A \wedge B)$

\begin{footnotesize}
\begin{oltableau}
[\pFmla{\False}{(\Diamond A \wedge \Diamond B) \rightarrow \Diamond (A \wedge B)}{1}, just = \TAss,
  [\pFmla{\True}{\Diamond A \wedge \Diamond B}{1}, just = {\TRule{\False}{\rightarrow}[1]},
    [\pFmla{\False}{\Diamond (A \wedge B)}{1}, just = {\TRule{\False}{\rightarrow}[1]}
      [\pFmla{\True}{\Diamond A}{1}, just = {\TRule{\True}{\wedge}[2]}
        [\pFmla{\True}{\Diamond B}{1}, just = {\TRule{\True}{\wedge}[2]}
          [\pFmla{\True}{A}{1.1}, just = {\TRule{\True}{\Diamond}[4]}
            [\pFmla{\False}{A \wedge B}{1.1}, just = {\TRule{\False}{\Diamond}[3]}
              [\pFmla{\False}{A}{1.1}, just = {\TRule{\False}{\wedge}[7]}, close]
              [\pFmla{\False}{B}{1.1}, just = {\TRule{\False}{\wedge}[7]}
                  [\pFmla{\True}{B}{1.2}, just = {\TRule{\True}{\Diamond}[5]}
                    [\pFmla{\False}{A \wedge B}{1.2}, just = {\TRule{\False}{\Diamond}[3]}
                      [\pFmla{\False}{A}{1.2}, just = {\TRule{\False}{\wedge}[7]}]
                      [\pFmla{\False}{B}{1.2}, just = {\TRule{\False}{\wedge}[7]}, close]
                    ]
                  ]
              ]
            ]
          ]
        ]
      ]
    ]
  ]
]
\end{oltableau}
And we're done. All the rules have been applied - though you really need to check this - and the middle branch does not close.
\end{footnotesize}

## A Model

When the tableau doesn't close, you should be able to build a model where the sentence is false at $w_1$.

In fact, you should be able to read it off the tree.

## A Model 

- Three worlds, $w_1, w_{1.1}, w_{1.2}$.
- The only accessibility relations are $w_1Rw_{1.1}$ and $w_1Rw_{1.2}$.
- In general, the accessibility relations are the ones required by the restrictions (but there are none here), plus the ones required by the numbering, i.e., $w_xRw_{x.y}$.
- $A$ is true at $w_{1.1}$ and false at $w_{1.2}$.
- $B$ is true at $w_{1.2}$ and false at $w_{1.1}$.
- It doesn't matter what atomics are true at $w_1$.
- But both $\Diamond A$ and $\Diamond B$ will be true at $w_1$, while $\Diamond (A \wedge B)$ is false there.

# $\neg \Box (A \wedge \neg \Box A)$ (in KT)


## Hypothesis

$\neg \Box (A \wedge \neg \Box A)$ is a theorem of KT.

- So we can use all the rules, plus the special rules for T.

## $\neg \Box (A \wedge \neg \Box A)$

\begin{oltableau}
[\pFmla{\False}{\neg \Box (A \wedge \neg \Box A)}{1}, just = \TAss,
]
\end{oltableau}

\bigskip

Start with it being false at 1.

## $\neg \Box (A \wedge \neg \Box A)$

\begin{oltableau}
[\pFmla{\False}{\neg \Box (A \wedge \neg \Box A)}{1}, just = \TAss,
  [\pFmla{\True}{\neg \neg \Box (A \wedge \neg \Box A)}{1}, just = {\TRule{\False}{\neg}[1]}
  ]
]
\end{oltableau}

\bigskip

Turn false $\neg$ false into true $\neg \neg$

## $\neg \Box (A \wedge \neg \Box A)$

\begin{oltableau}
[\pFmla{\False}{\neg \Box (A \wedge \neg \Box A)}{1}, just = \TAss,
  [\pFmla{\True}{\neg \neg \Box (A \wedge \neg \Box A)}{1}, just = {\TRule{\False}{\neg}[1]}
    [\pFmla{\True}{\Box (A \wedge \neg \Box A)}{1}, just = {\TRule{\True}{\neg}[2]}
    ]
  ]
]
\end{oltableau}

\bigskip

Delete $\neg \neg$

## $\neg \Box (A \wedge \neg \Box A)$

\begin{oltableau}
[\pFmla{\False}{\neg \Box (A \wedge \neg \Box A)}{1}, just = \TAss,
  [\pFmla{\True}{\neg \neg \Box (A \wedge \neg \Box A)}{1}, just = {\TRule{\False}{\neg}[1]}
    [\pFmla{\True}{\Box (A \wedge \neg \Box A)}{1}, just = {\TRule{\True}{\neg}[2]}
      [\pFmla{\True}{A \wedge \neg \Box A}{1}, just = {T $\Box$ 2}
      ]    
    ]
  ]
]
\end{oltableau}

\bigskip

It's KT, so whatever is necessary is true.

## $\neg \Box (A \wedge \neg \Box A)$

\begin{oltableau}
[\pFmla{\False}{\neg \Box (A \wedge \neg \Box A)}{1}, just = \TAss,
  [\pFmla{\True}{\neg \neg \Box (A \wedge \neg \Box A)}{1}, just = {\TRule{\False}{\neg}[1]}
    [\pFmla{\True}{\Box (A \wedge \neg \Box A)}{1}, just = {\TRule{\True}{\neg}[2]}
      [\pFmla{\True}{A \wedge \neg \Box A}{1}, just = {T $\Box$ 2}
        [\pFmla{\True}{A}{1}, just = {\TRule{\True}{\wedge}[4]}
          [\pFmla{\True}{\neg \Box A}{1}, just = {\TRule{\True}{\wedge}[4]}
          ]
        ]
      ]    
    ]
  ]
]
\end{oltableau}

\bigskip

Both sides of a conjunction have to be true.

## $\neg \Box (A \wedge \neg \Box A)$

\begin{oltableau}
[\pFmla{\False}{\neg \Box (A \wedge \neg \Box A)}{1}, just = \TAss,
  [\pFmla{\True}{\neg \neg \Box (A \wedge \neg \Box A)}{1}, just = {\TRule{\False}{\neg}[1]}
    [\pFmla{\True}{\Box (A \wedge \neg \Box A)}{1}, just = {\TRule{\True}{\neg}[2]}
      [\pFmla{\True}{A \wedge \neg \Box A}{1}, just = {T $\Box$ 2}
        [\pFmla{\True}{A}{1}, just = {\TRule{\True}{\wedge}[4]}
          [\pFmla{\True}{\neg \Box A}{1}, just = {\TRule{\True}{\wedge}[4]}
            [\pFmla{\False}{\Box A}{1}, just = {\TRule{\False}{\neg}[6]}
            ]
          ]
        ]
      ]    
    ]
  ]
]
\end{oltableau}

\bigskip

Whatever isn't true is false.

## $\neg \Box (A \wedge \neg \Box A)$

\begin{oltableau}
[\pFmla{\False}{\neg \Box (A \wedge \neg \Box A)}{1}, just = \TAss,
  [\pFmla{\True}{\neg \neg \Box (A \wedge \neg \Box A)}{1}, just = {\TRule{\False}{\neg}[1]}
    [\pFmla{\True}{\Box (A \wedge \neg \Box A)}{1}, just = {\TRule{\True}{\neg}[2]}
      [\pFmla{\True}{A \wedge \neg \Box A}{1}, just = {T $\Box$ 2}
        [\pFmla{\True}{A}{1}, just = {\TRule{\True}{\wedge}[4]}
          [\pFmla{\True}{\neg \Box A}{1}, just = {\TRule{\True}{\wedge}[4]}
            [\pFmla{\False}{\Box A}{1}, just = {\TRule{\False}{\neg}[6]}
              [\pFmla{\False}{A}{1.1}, just = {\TRule{\False}{\Box}[7]}
              ]
            ]
          ]
        ]
      ]    
    ]
  ]
]
\end{oltableau}

\bigskip

A false Box sentence requires a world that makes it false. What can we do now?

## $\neg \Box (A \wedge \neg \Box A)$

\begin{oltableau}
[\pFmla{\False}{\neg \Box (A \wedge \neg \Box A)}{1}, just = \TAss,
  [\pFmla{\True}{\neg \neg \Box (A \wedge \neg \Box A)}{1}, just = {\TRule{\False}{\neg}[1]}
    [\pFmla{\True}{\Box (A \wedge \neg \Box A)}{1}, just = {\TRule{\True}{\neg}[2]}
      [\pFmla{\True}{A \wedge \neg \Box A}{1}, just = {T $\Box$ 2}
        [\pFmla{\True}{A}{1}, just = {\TRule{\True}{\wedge}[4]}
          [\pFmla{\True}{\neg \Box A}{1}, just = {\TRule{\True}{\wedge}[4]}
            [\pFmla{\False}{\Box A}{1}, just = {\TRule{\False}{\neg}[6]}
              [\pFmla{\False}{A}{1.1}, just = {\TRule{\False}{\Box}[7]}
                [\pFmla{\True}{A \wedge \neg \Box A}{1.1}, just = {\TRule{\True}{\Box}[3]}
                ]
              ]
            ]
          ]
        ]
      ]    
    ]
  ]
]
\end{oltableau}

Line 3 is a $\Box$ sentence, so the unboxed part applies everywhere accessible.

## $\neg \Box (A \wedge \neg \Box A)$

\begin{oltableau}
[\pFmla{\False}{\neg \Box (A \wedge \neg \Box A)}{1}, just = \TAss,
  [\pFmla{\True}{\neg \neg \Box (A \wedge \neg \Box A)}{1}, just = {\TRule{\False}{\neg}[1]}
    [\pFmla{\True}{\Box (A \wedge \neg \Box A)}{1}, just = {\TRule{\True}{\neg}[2]}
      [\pFmla{\True}{A \wedge \neg \Box A}{1}, just = {T $\Box$ 2}
        [\pFmla{\True}{A}{1}, just = {\TRule{\True}{\wedge}[4]}
          [\pFmla{\True}{\neg \Box A}{1}, just = {\TRule{\True}{\wedge}[4]}
            [\pFmla{\False}{\Box A}{1}, just = {\TRule{\False}{\neg}[6]}
              [\pFmla{\False}{A}{1.1}, just = {\TRule{\False}{\Box}[7]}
                [\pFmla{\True}{A \wedge \neg \Box A}{1.1}, just = {\TRule{\True}{\Box}[3]}
                  [\pFmla{\True}{A}{1.1}, just = {\TRule{\True}{\wedge}[9]}, close
                  ]
                ]
              ]
            ]
          ]
        ]
      ]    
    ]
  ]
]
\end{oltableau}

And both parts of an and sentence have to be true - though the first is enough to close this tree.

## Philosophical Consequences

- This is a philosophically interesting result.
- If $\Box$ means "Is known by X", then it says that X can't know of a particular proposition that it is true but they don't know it.
- Assuming that X is not omniscient, so there are some things they don't know, this means there are limits to X's knowledge.

## Idealism

- Let B = "Brian doesn't know that B is true". (And assume, for now, that this kind of self-reference makes sense.
- That's surely true. My knowing it implies a contradiction in the way we've just shown.
- So we all know it, because we can all follow the proof. $\pause$
- Except wait - it's true, and it says I don't know it, so I must not know it.
- So there's something you all know that I don't know.
- Though just why I don't know it is something of a mystery, since I do have a well-supported (and correct) belief that it is true.

# $\Box A \rightarrow \Box \Box A$ (in KT)


## Hypothesis

$\Box A \rightarrow \Box \Box A$ is a theorem of KT.

- So we can use all the rules, plus the special rules for T.

## $\Box A \rightarrow \Box \Box A$

\begin{oltableau}
[\pFmla{\False}{\Box A \rightarrow \Box \Box A}{1}, just = \TAss,
]
\end{oltableau}

\bigskip

Start with it being false at 1.

## $\Box A \rightarrow \Box \Box A$

\begin{oltableau}
[\pFmla{\False}{\Box A \rightarrow \Box \Box A}{1}, just = \TAss
  [\pFmla{\True}{\Box A}{1}, just = {\TRule{\False}{\rightarrow}[1]}
    [\pFmla{\False}{\Box \Box A}{1}, just = {\TRule{\False}{\rightarrow}[1]}
    ]
  ]
]
\end{oltableau}

\bigskip

You know the drill - left hand side true, right hand side false.

## $\Box A \rightarrow \Box \Box A$

\begin{oltableau}
[\pFmla{\False}{\Box A \rightarrow \Box \Box A}{1}, just = \TAss
  [\pFmla{\True}{\Box A}{1}, just = {\TRule{\False}{\rightarrow}[1]}
    [\pFmla{\False}{\Box \Box A}{1}, just = {\TRule{\False}{\rightarrow}[1]}
      [\pFmla{\True}{A}{1}, just = {T $\Box$ 2}
      ]
    ]
  ]
]
\end{oltableau}

\bigskip

It's T, so we have obligations when a $\Box$ sentence is true.

## $\Box A \rightarrow \Box \Box A$

\begin{oltableau}
[\pFmla{\False}{\Box A \rightarrow \Box \Box A}{1}, just = \TAss
  [\pFmla{\True}{\Box A}{1}, just = {\TRule{\False}{\rightarrow}[1]}
    [\pFmla{\False}{\Box \Box A}{1}, just = {\TRule{\False}{\rightarrow}[1]}
      [\pFmla{\True}{A}{1}, just = {T $\Box$ 2}
        [\pFmla{\False}{\Box A}{1.1}, just = {\TRule{\False}{\Box}[3]}
        ]
      ]
    ]
  ]
]
\end{oltableau}

\bigskip

Now we have to make the false $\Box$ sentence actually false.

## $\Box A \rightarrow \Box \Box A$

\begin{oltableau}
[\pFmla{\False}{\Box A \rightarrow \Box \Box A}{1}, just = \TAss
  [\pFmla{\True}{\Box A}{1}, just = {\TRule{\False}{\rightarrow}[1]}
    [\pFmla{\False}{\Box \Box A}{1}, just = {\TRule{\False}{\rightarrow}[1]}
      [\pFmla{\True}{A}{1}, just = {T $\Box$ 2}
        [\pFmla{\False}{\Box A}{1.1}, just = {\TRule{\False}{\Box}[3]}
          [\pFmla{\True}{A}{1.1}, just = {\TRule{\True}{\Box}[2]}        
          ]
        ]
      ]
    ]
  ]
]
\end{oltableau}

\bigskip

Carry down the true $\Box$ sentence.

## $\Box A \rightarrow \Box \Box A$

\begin{oltableau}
[\pFmla{\False}{\Box A \rightarrow \Box \Box A}{1}, just = \TAss
  [\pFmla{\True}{\Box A}{1}, just = {\TRule{\False}{\rightarrow}[1]}
    [\pFmla{\False}{\Box \Box A}{1}, just = {\TRule{\False}{\rightarrow}[1]}
      [\pFmla{\True}{A}{1}, just = {T $\Box$ 2}
        [\pFmla{\False}{\Box A}{1.1}, just = {\TRule{\False}{\Box}[3]}
          [\pFmla{\True}{A}{1.1}, just = {\TRule{\True}{\Box}[2]}        
            [\pFmla{\False}{A}{1.1.1}, just = {\TRule{\False}{\Box}[5]}
            ]
          ]
        ]
      ]
    ]
  ]
]
\end{oltableau}

\bigskip

- One more false $\Box$ sentence. \pause
- And now we're done; all rules applied, and tree open. So it is not a theorem.

## A Model 

- Three worlds, $w_1, w_{1.1}, w_{1.1.1}$.
- The accessibility relations are $w_1Rw_{1.1}, w_{1.1}Rw_{1.1.1}, w_1Rw_1, w_{1.1}Rw_{1.1}$ and $w_{1.1.1}Rw_{1.1.1}$.
- The first two are from the tree, the next three from the restriction.
- $A$ is true at $w_1$ and $w_{1.1}$ and false at $w_{1.1.1}$.
- So $\Box A$ will be true only at $w_1$.
- So $\Box \Box A$ will be false at $w_1$, as required.

# $\Box A \rightarrow (A \wedge \Box \Box A)$ (in S4)


## Hypothesis

$\Box A \rightarrow (A \wedge \Box \Box A)$ is a theorem of S4 = KT4.

- So we can use all the rules, plus the special rules for T and for 4.

## $\Box A \rightarrow (A \wedge \Box \Box A)$

\begin{oltableau}
[\pFmla{\False}{\Box A \rightarrow (A \wedge \Box \Box A)}{1}, just = \TAss,
]
\end{oltableau}

\bigskip

Start with it being false at 1.

## $\Box A \rightarrow \Box \Box A$

\begin{oltableau}
[\pFmla{\False}{\Box A \rightarrow (A \wedge \Box \Box A)}{1}, just = \TAss
  [\pFmla{\True}{\Box A}{1}, just = {\TRule{\False}{\rightarrow}[1]}
    [\pFmla{\False}{A \wedge \Box \Box A}{1}, just = {\TRule{\False}{\rightarrow}[1]}
    ]
  ]
]
\end{oltableau}

\bigskip

You know the drill - left hand side true, right hand side false.

## $\Box A \rightarrow \Box \Box A$

\begin{oltableau}
[\pFmla{\False}{\Box A \rightarrow (A \wedge \Box \Box A)}{1}, just = \TAss
  [\pFmla{\True}{\Box A}{1}, just = {\TRule{\False}{\rightarrow}[1]}
    [\pFmla{\False}{A \wedge \Box \Box A}{1}, just = {\TRule{\False}{\rightarrow}[1]}
      [\pFmla{\True}{A}{1}, just = {T $\Box$ 2}
      ]
    ]
  ]
]
\end{oltableau}

\bigskip

We have T, so necessary truths are true.

## $\Box A \rightarrow \Box \Box A$

\begin{oltableau}
[\pFmla{\False}{\Box A \rightarrow (A \wedge \Box \Box A)}{1}, just = \TAss
  [\pFmla{\True}{\Box A}{1}, just = {\TRule{\False}{\rightarrow}[1]}
    [\pFmla{\False}{A \wedge \Box \Box A}{1}, just = {\TRule{\False}{\rightarrow}[1]}
      [\pFmla{\True}{A}{1}, just = {T $\Box$ 2}
        [\pFmla{\False}{A}{1}, just = {\TRule{\False}{\wedge}[3]}, close]
        [\pFmla{\False}{\Box \Box A}{1}, just = {\TRule{\False}{\wedge}[3]}
        ]
      ]
    ]
  ]
]
\end{oltableau}

\bigskip

False $\wedge$ means branching, but happily one branch closes immediately.

## $\Box A \rightarrow \Box \Box A$

\begin{oltableau}
[\pFmla{\False}{\Box A \rightarrow (A \wedge \Box \Box A)}{1}, just = \TAss
  [\pFmla{\True}{\Box A}{1}, just = {\TRule{\False}{\rightarrow}[1]}
    [\pFmla{\False}{A \wedge \Box \Box A}{1}, just = {\TRule{\False}{\rightarrow}[1]}
      [\pFmla{\True}{A}{1}, just = {T $\Box$ 2}
        [\pFmla{\False}{A}{1}, just = {\TRule{\False}{\wedge}[3]}, close]
        [\pFmla{\False}{\Box \Box A}{1}, just = {\TRule{\False}{\wedge}[3]}
          [\pFmla{\False}{\Box A}{1.1}, just = {\TRule{\False}{\Box}[5]}
          ]
        ]
      ]
    ]
  ]
]
\end{oltableau}

\bigskip

False $\Box$ sentences require new worlds where the unboxed thing is false.

## $\Box A \rightarrow \Box \Box A$

\begin{oltableau}
[\pFmla{\False}{\Box A \rightarrow (A \wedge \Box \Box A)}{1}, just = \TAss
  [\pFmla{\True}{\Box A}{1}, just = {\TRule{\False}{\rightarrow}[1]}
    [\pFmla{\False}{A \wedge \Box \Box A}{1}, just = {\TRule{\False}{\rightarrow}[1]}
      [\pFmla{\True}{A}{1}, just = {T $\Box$ 2}
        [\pFmla{\False}{A}{1}, just = {\TRule{\False}{\wedge}[3]}, close]
        [\pFmla{\False}{\Box \Box A}{1}, just = {\TRule{\False}{\wedge}[3]}
          [\pFmla{\False}{\Box A}{1.1}, just = {\TRule{\False}{\Box}[5]}
            [\pFmla{\True}{\Box A}{1.1}, just = {4 $\Box$ 2}, close]
          ]
        ]
      ]
    ]
  ]
]
\end{oltableau}

\bigskip

But 4 requires we carry down $\Box$ sentences, and now we're done.



# $A \rightarrow \Box \Diamond A$ (in S4)


## Hypothesis

$A \rightarrow \Box \Diamond A$ is a theorem of S4 = KT4.

- So we can use all the rules, plus the special rules for T and for 4.

## $A \rightarrow \Box \Diamond A$

\begin{oltableau}
[\pFmla{\False}{A \rightarrow \Box \Diamond A}{1}, just = \TAss,
]
\end{oltableau}

\bigskip

Start with it being false at 1.

## $A \rightarrow \Box \Diamond A$

\begin{oltableau}
[\pFmla{\False}{A \rightarrow \Box \Diamond A}{1}, just = \TAss
  [\pFmla{\True}{A}{1}, just = {\TRule{\False}{\rightarrow}[1]}
    [\pFmla{\False}{\Box \Diamond A}{1}, just = {\TRule{\False}{\rightarrow}[1]}
    ]
  ]
]
\end{oltableau}

\bigskip

You know the drill - left hand side true, right hand side false.

## $A \rightarrow \Box \Diamond A$

\begin{oltableau}
[\pFmla{\False}{A \rightarrow \Box \Diamond A}{1}, just = \TAss
  [\pFmla{\True}{A}{1}, just = {\TRule{\False}{\rightarrow}[1]}
    [\pFmla{\False}{\Box \Diamond A}{1}, just = {\TRule{\False}{\rightarrow}[1]}
      [\pFmla{\False}{\Diamond A}{1.1}, just = {\TRule{\False}{\Box}[3]}
      ]
    ]
  ]
]
\end{oltableau}

\bigskip

False $\Box$ sentences are false somewhere.

## $A \rightarrow \Box \Diamond A$

\begin{oltableau}
[\pFmla{\False}{A \rightarrow \Box \Diamond A}{1}, just = \TAss
  [\pFmla{\True}{A}{1}, just = {\TRule{\False}{\rightarrow}[1]}
    [\pFmla{\False}{\Box \Diamond A}{1}, just = {\TRule{\False}{\rightarrow}[1]}
      [\pFmla{\False}{\Diamond A}{1.1}, just = {\TRule{\False}{\Box}[3]}
        [\pFmla{\False}{A}{1.1}, just = {T $\Diamond$ 4}]
      ]
    ]
  ]
]
\end{oltableau}

\bigskip

It's T, so false $\Diamond$ sentences have to actually be false.

## $A \rightarrow \Box \Diamond A$

\begin{oltableau}
[\pFmla{\False}{A \rightarrow \Box \Diamond A}{1}, just = \TAss
  [\pFmla{\True}{A}{1}, just = {\TRule{\False}{\rightarrow}[1]}
    [\pFmla{\False}{\Box \Diamond A}{1}, just = {\TRule{\False}{\rightarrow}[1]}
      [\pFmla{\False}{\Diamond A}{1.1}, just = {\TRule{\False}{\Box}[3]}
        [\pFmla{\False}{A}{1.1}, just = {T $\Diamond$ 4}]
      ]
    ]
  ]
]
\end{oltableau}

\bigskip

- But that's it 
- We've applied all the rules, and it doesn't close.
- So not a theorem.

## A Model 

- Two worlds, $w_1, w_{1.1}$.
- The accessibility relations are $w_1Rw_{1.1}, w_1Rw_1$ and $w_{1.1}Rw_{1.1}$.
- The first is from the tree, the next two from reflexivity.
- In this case, transitivity doesn't require anything more. (Though double check this!)
- $A$ is true at $w_1$ and and false at $w_{1.1}$.
- So $\Diamond A$ will be false only at $w_{1.1}$.
- So $\Box \Diamond A$ will be false at $w_1$, while $A$ is true, as required.


# $A \rightarrow \Box \Diamond A$ (in KTB)


## Hypothesis

$A \rightarrow \Box \Diamond A$ is a theorem of KTB.

- So we can use all the rules, plus the special rules for B and T.

## $A \rightarrow \Box \Diamond A$

\begin{oltableau}
[\pFmla{\False}{A \rightarrow \Box \Diamond A}{1}, just = \TAss,
]
\end{oltableau}

\bigskip

Start with it being false at 1.

## $A \rightarrow \Box \Diamond A$

\begin{oltableau}
[\pFmla{\False}{A \rightarrow \Box \Diamond A}{1}, just = \TAss
  [\pFmla{\True}{A}{1}, just = {\TRule{\False}{\rightarrow}[1]}
    [\pFmla{\False}{\Box \Diamond A}{1}, just = {\TRule{\False}{\rightarrow}[1]}
    ]
  ]
]
\end{oltableau}

\bigskip

You know the drill - left hand side true, right hand side false.

## $A \rightarrow \Box \Diamond A$

\begin{oltableau}
[\pFmla{\False}{A \rightarrow \Box \Diamond A}{1}, just = \TAss
  [\pFmla{\True}{A}{1}, just = {\TRule{\False}{\rightarrow}[1]}
    [\pFmla{\False}{\Box \Diamond A}{1}, just = {\TRule{\False}{\rightarrow}[1]}
      [\pFmla{\False}{\Diamond A}{1.1}, just = {\TRule{\False}{\Box}[3]}
      ]
    ]
  ]
]
\end{oltableau}

\bigskip

False $\Box$ sentences are false somewhere.

## $A \rightarrow \Box \Diamond A$

\begin{oltableau}
[\pFmla{\False}{A \rightarrow \Box \Diamond A}{1}, just = \TAss
  [\pFmla{\True}{A}{1}, just = {\TRule{\False}{\rightarrow}[1]}
    [\pFmla{\False}{\Box \Diamond A}{1}, just = {\TRule{\False}{\rightarrow}[1]}
      [\pFmla{\False}{\Diamond A}{1.1}, just = {\TRule{\False}{\Box}[3]}
        [\pFmla{\False}{A}{1}, just = {B $\Diamond$ 4}]
      ]
    ]
  ]
]
\end{oltableau}

\bigskip

In B, false $\Diamond$ sentences have to be false one step backwards as well as one step forwards.

## $A \rightarrow \Box \Diamond A$

\begin{oltableau}
[\pFmla{\False}{A \rightarrow \Box \Diamond A}{1}, just = \TAss
  [\pFmla{\True}{A}{1}, just = {\TRule{\False}{\rightarrow}[1]}
    [\pFmla{\False}{\Box \Diamond A}{1}, just = {\TRule{\False}{\rightarrow}[1]}
      [\pFmla{\False}{\Diamond A}{1.1}, just = {\TRule{\False}{\Box}[3]}
        [\pFmla{\False}{A}{1}, just = {B $\Diamond$ 4}, close]
      ]
    ]
  ]
]
\end{oltableau}

\bigskip

And that closes the tree, so it is a theorem.


# $\Box A \rightarrow \Box \Box A$ (in KTB)


## Hypothesis

$\Box A \rightarrow \Box \Box A$ is a theorem of KTB.

- So we can use all the rules, plus the special rules for B.

## $\Box A \rightarrow \Box \Box A$

\begin{oltableau}
[\pFmla{\False}{\Box A \rightarrow \Box \Box A}{1}, just = \TAss,
]
\end{oltableau}

\bigskip

Start with it being false at 1.

## $\Box A \rightarrow \Box \Box A$

\begin{oltableau}
[\pFmla{\False}{\Box A \rightarrow \Box \Box A}{1}, just = \TAss
  [\pFmla{\True}{\Box A}{1}, just = {\TRule{\False}{\rightarrow}[1]}
    [\pFmla{\False}{\Box \Box A}{1}, just = {\TRule{\False}{\rightarrow}[1]}
    ]
  ]
]
\end{oltableau}

\bigskip

You know the drill - left hand side true, right hand side false.

## $\Box A \rightarrow \Box \Box A$

\begin{oltableau}
[\pFmla{\False}{\Box A \rightarrow \Box \Box A}{1}, just = \TAss
  [\pFmla{\True}{\Box A}{1}, just = {\TRule{\False}{\rightarrow}[1]}
    [\pFmla{\False}{\Box \Box A}{1}, just = {\TRule{\False}{\rightarrow}[1]}
      [\pFmla{\True}{A}{1}, just = {T $\Box$ 2}
      ]
    ]
  ]
]
\end{oltableau}

\bigskip

It's T, so true box sentences are true.

## $\Box A \rightarrow \Box \Box A$

\begin{oltableau}
[\pFmla{\False}{\Box A \rightarrow \Box \Box A}{1}, just = \TAss
  [\pFmla{\True}{\Box A}{1}, just = {\TRule{\False}{\rightarrow}[1]}
    [\pFmla{\False}{\Box \Box A}{1}, just = {\TRule{\False}{\rightarrow}[1]}
      [\pFmla{\True}{A}{1}, just = {T $\Box$ 2}
        [\pFmla{\False}{\Box A}{1.1}, just = {\TRule{\False}{\Box}[3]}
        ]
      ]
    ]
  ]
]
\end{oltableau}

\bigskip

False $\Box$ sentences have to be false somewhere.

## $\Box A \rightarrow \Box \Box A$

\begin{oltableau}
[\pFmla{\False}{\Box A \rightarrow \Box \Box A}{1}, just = \TAss
  [\pFmla{\True}{\Box A}{1}, just = {\TRule{\False}{\rightarrow}[1]}
    [\pFmla{\False}{\Box \Box A}{1}, just = {\TRule{\False}{\rightarrow}[1]}
      [\pFmla{\True}{A}{1}, just = {T $\Box$ 2}
        [\pFmla{\False}{\Box A}{1.1}, just = {\TRule{\False}{\Box}[3]}
          [\pFmla{\True}{A}{1.1}, just = {\TRule{\True}{\Box}[2]}
          ]
        ]
      ]
    ]
  ]
]
\end{oltableau}

\bigskip

True $\Box$ sentences have to be true everywhere accessible.

## $\Box A \rightarrow \Box \Box A$

\begin{oltableau}
[\pFmla{\False}{\Box A \rightarrow \Box \Box A}{1}, just = \TAss
  [\pFmla{\True}{\Box A}{1}, just = {\TRule{\False}{\rightarrow}[1]}
    [\pFmla{\False}{\Box \Box A}{1}, just = {\TRule{\False}{\rightarrow}[1]}
      [\pFmla{\True}{A}{1}, just = {T $\Box$ 2}
        [\pFmla{\False}{\Box A}{1.1}, just = {\TRule{\False}{\Box}[3]}
          [\pFmla{\True}{A}{1.1}, just = {\TRule{\True}{\Box}[2]}
            [\pFmla{\False}{A}{1.1.1}, just = {\TRule{\False}{\Box}[5]}
            ]
          ]
        ]
      ]
    ]
  ]
]
\end{oltableau}

\bigskip

Another false $\Box$ sentence that needs to be made false.


## $\Box A \rightarrow \Box \Box A$

\begin{oltableau}
[\pFmla{\False}{\Box A \rightarrow \Box \Box A}{1}, just = \TAss
  [\pFmla{\True}{\Box A}{1}, just = {\TRule{\False}{\rightarrow}[1]}
    [\pFmla{\False}{\Box \Box A}{1}, just = {\TRule{\False}{\rightarrow}[1]}
      [\pFmla{\True}{A}{1}, just = {T $\Box$ 2}
        [\pFmla{\False}{\Box A}{1.1}, just = {\TRule{\False}{\Box}[3]}
          [\pFmla{\True}{A}{1.1}, just = {\TRule{\True}{\Box}[2]}
            [\pFmla{\False}{A}{1.1.1}, just = {\TRule{\False}{\Box}[5]}
            ]
          ]
        ]
      ]
    ]
  ]
]
\end{oltableau}

\bigskip

And that's it. We've applied all the rules. The extra rules for T and B don't change much here from the basic tableau in K.

## A Model 

- Three worlds, $w_1, w_{1.1}, w_{1.1.1}$.
- The accessibility relations are $w_1Rw_{1.1}, w_{1.1}Rw_{1.1.1}, w_1Rw_1, w_{1.1}Rw_{1.1}, w_{1.1.1}Rw_{1.1.1}, w_{1.1}Rw_1$ and $w_{1.1.1}Rw_{1.1}$
- The first two are from the tree, the next three from T and the last two from B.
- $A$ is true at $w_1$ and $w_{1.1}$ and false at $w_{1.1.1}$.
- So $\Box A$ will be true only at $w_1$.
- So $\Box \Box A$ will be false at $w_1$, as required.


# $\Box(\Box A \rightarrow B) \vee \Box(\Box B \rightarrow A)$ (in S4)


## Hypothesis

$\Box(\Box A \rightarrow B) \vee \Box(\Box B \rightarrow A)$ is a theorem of S4.

- So we can use all the rules, plus the special rules for T and 4.

## $\Box(\Box A \rightarrow B) \vee \Box(\Box B \rightarrow A)$

\begin{oltableau}
[\pFmla{\False}{\Box(\Box A \rightarrow B) \vee \Box(\Box B \rightarrow A)}{1}, just = \TAss,
]
\end{oltableau}

\bigskip

Start with it being false at 1.

## $\Box(\Box A \rightarrow B) \vee \Box(\Box B \rightarrow A)$

\begin{oltableau}
[\pFmla{\False}{\Box(\Box A \rightarrow B) \vee \Box(\Box B \rightarrow A)}{1}, just = \TAss,
  [\pFmla{\False}{\Box(\Box A \rightarrow B)}{1}, just = {\TRule{\False}{\vee}[1]}
    [\pFmla{\False}{\Box(\Box B \rightarrow A)}{1}, just = {\TRule{\False}{\vee}[1]}
    ]
  ]
]
\end{oltableau}

\bigskip

False $\vee$ sentences have both sides false.

## $\Box(\Box A \rightarrow B) \vee \Box(\Box B \rightarrow A)$

\begin{oltableau}
[\pFmla{\False}{\Box(\Box A \rightarrow B) \vee \Box(\Box B \rightarrow A)}{1}, just = \TAss,
  [\pFmla{\False}{\Box(\Box A \rightarrow B)}{1}, just = {\TRule{\False}{\vee}[1]}
    [\pFmla{\False}{\Box(\Box B \rightarrow A)}{1}, just = {\TRule{\False}{\vee}[1]}
      [\pFmla{\False}{\Box A \rightarrow B}{1.1}, just = {\TRule{\False}{\Box}[2]}
        [\pFmla{\False}{\Box B \rightarrow A}{1.2}, just = {\TRule{\False}{\Box}[3]}
        ]
      ]
    ]
  ]
]
\end{oltableau}

\bigskip

Both of these false $\Box$ sentences have to be made false somehow.

## $\Box(\Box A \rightarrow B) \vee \Box(\Box B \rightarrow A)$

\begin{oltableau}
[\pFmla{\False}{\Box(\Box A \rightarrow B) \vee \Box(\Box B \rightarrow A)}{1}, just = \TAss,
  [\pFmla{\False}{\Box(\Box A \rightarrow B)}{1}, just = {\TRule{\False}{\vee}[1]}
    [\pFmla{\False}{\Box(\Box B \rightarrow A)}{1}, just = {\TRule{\False}{\vee}[1]}
      [\pFmla{\False}{\Box A \rightarrow B}{1.1}, just = {\TRule{\False}{\Box}[2]}
        [\pFmla{\False}{\Box B \rightarrow A}{1.2}, just = {\TRule{\False}{\Box}[3]}
          [\pFmla{\True}{\Box A}{1.1}, just = {\TRule{\False}{\rightarrow}[4]}
            [\pFmla{\False}{B}{1.1}, just = {\TRule{\False}{\rightarrow}[4]}
              [\pFmla{\True}{\Box B}{1.2}, just = {\TRule{\False}{\rightarrow}[5]}
                [\pFmla{\False}{A}{1.2}, just = {\TRule{\False}{\rightarrow}[5]}
                ]
              ]
            ]
          ]
        ]
      ]
    ]
  ]
]
\end{oltableau}

\bigskip

- False $\rightarrow$ sentences mean left false; right true.
- Note we have no special rules for 4 or T triggered yet, because no true $\Box$ or false $\Diamond$, but that's about to change.

## $\Box(\Box A \rightarrow B) \vee \Box(\Box B \rightarrow A)$

\begin{oltableau}
[\pFmla{\False}{\Box(\Box A \rightarrow B) \vee \Box(\Box B \rightarrow A)}{1}, just = \TAss,
  [\pFmla{\False}{\Box(\Box A \rightarrow B)}{1}, just = {\TRule{\False}{\vee}[1]}
    [\pFmla{\False}{\Box(\Box B \rightarrow A)}{1}, just = {\TRule{\False}{\vee}[1]}
      [\pFmla{\False}{\Box A \rightarrow B}{1.1}, just = {\TRule{\False}{\Box}[2]}
        [\pFmla{\False}{\Box B \rightarrow A}{1.2}, just = {\TRule{\False}{\Box}[3]}
          [\pFmla{\True}{\Box A}{1.1}, just = {\TRule{\False}{\rightarrow}[4]}
            [\pFmla{\False}{B}{1.1}, just = {\TRule{\False}{\rightarrow}[4]}
              [\pFmla{\True}{\Box B}{1.2}, just = {\TRule{\False}{\rightarrow}[5]}
                [\pFmla{\False}{A}{1.2}, just = {\TRule{\False}{\rightarrow}[5]}
                  [\pFmla{\True}{A}{1.1}, just = {T $\Box$ 6}
                    [\pFmla{\True}{B}{1.2}, just = {T $\Box$ 8}
                    ]
                  ]
                ]
              ]
            ]
          ]
        ]
      ]
    ]
  ]
]
\end{oltableau}

\bigskip

T means true $\Box$ sentences are true unboxed.

## $\Box(\Box A \rightarrow B) \vee \Box(\Box B \rightarrow A)$

\begin{oltableau}
[\pFmla{\False}{\Box(\Box A \rightarrow B) \vee \Box(\Box B \rightarrow A)}{1}, just = \TAss,
  [\pFmla{\False}{\Box(\Box A \rightarrow B)}{1}, just = {\TRule{\False}{\vee}[1]}
    [\pFmla{\False}{\Box(\Box B \rightarrow A)}{1}, just = {\TRule{\False}{\vee}[1]}
      [\pFmla{\False}{\Box A \rightarrow B}{1.1}, just = {\TRule{\False}{\Box}[2]}
        [\pFmla{\False}{\Box B \rightarrow A}{1.2}, just = {\TRule{\False}{\Box}[3]}
          [\pFmla{\True}{\Box A}{1.1}, just = {\TRule{\False}{\rightarrow}[4]}
            [\pFmla{\False}{B}{1.1}, just = {\TRule{\False}{\rightarrow}[4]}
              [\pFmla{\True}{\Box B}{1.2}, just = {\TRule{\False}{\rightarrow}[5]}
                [\pFmla{\False}{A}{1.2}, just = {\TRule{\False}{\rightarrow}[5]}
                  [\pFmla{\True}{A}{1.1}, just = {T $\Box$ 6}
                    [\pFmla{\True}{B}{1.2}, just = {T $\Box$ 8}
                    ]
                  ]
                ]
              ]
            ]
          ]
        ]
      ]
    ]
  ]
]
\end{oltableau}

\bigskip

But now we've applied all the rules, and the tableau doesn't close. So not a theorem.

## A Model

- Three worlds, $w_1, w_{1.1}, w_{1.2}$
- The accessibility relations are $w_1Rw_{1.1}, w_1Rw{1.2}, w_1Rw_1, w_{1.1}Rw_{1.1}, w_{1.2}Rw_{1.2}$.
- The first two from the tree, the last three from T. Adding 4 doesn't require anything in this case.
- $A$ is true at $w_{1.1}$ and false at $w_{1.2}$.
- $B$ is true at $w_{1.2}$ and false at $w_{1.1}$.
- It doesn't matter what values the atomics take at $w_1$.
- So $\Box A$ will be true at $w_{1.1}$, while $B$ is false.
- And $\Box B$ will be true at $w_{1.2}$, while $A$ is false.
- So the original sentence fails at $w_1$.

# $\Box(\Box A \rightarrow B) \vee \Box(\Box B \rightarrow A)$ (in S5)


## Hypothesis

$\Box(\Box A \rightarrow B) \vee \Box(\Box B \rightarrow A)$ is a theorem of S5.

- We are going to use simplified S5 because normal S5 is really painful for cases like this one.

## $\Box(\Box A \rightarrow B) \vee \Box(\Box B \rightarrow A)$

\begin{oltableau}
[\pFmla{\False}{\Box(\Box A \rightarrow B) \vee \Box(\Box B \rightarrow A)}{1}, just = \TAss,
]
\end{oltableau}

\bigskip

Start with it being false at 1.

## $\Box(\Box A \rightarrow B) \vee \Box(\Box B \rightarrow A)$

\begin{oltableau}
[\pFmla{\False}{\Box(\Box A \rightarrow B) \vee \Box(\Box B \rightarrow A)}{1}, just = \TAss,
  [\pFmla{\False}{\Box(\Box A \rightarrow B)}{1}, just = {\TRule{\False}{\vee}[1]}
    [\pFmla{\False}{\Box(\Box B \rightarrow A)}{1}, just = {\TRule{\False}{\vee}[1]}
    ]
  ]
]
\end{oltableau}

\bigskip

False $\vee$ sentences have both sides false.

## $\Box(\Box A \rightarrow B) \vee \Box(\Box B \rightarrow A)$

\begin{oltableau}
[\pFmla{\False}{\Box(\Box A \rightarrow B) \vee \Box(\Box B \rightarrow A)}{1}, just = \TAss,
  [\pFmla{\False}{\Box(\Box A \rightarrow B)}{1}, just = {\TRule{\False}{\vee}[1]}
    [\pFmla{\False}{\Box(\Box B \rightarrow A)}{1}, just = {\TRule{\False}{\vee}[1]}
      [\pFmla{\False}{\Box A \rightarrow B}{2}, just = {\TRule{\False}{\Box}[2]}
        [\pFmla{\False}{\Box B \rightarrow A}{3}, just = {\TRule{\False}{\Box}[3]}
        ]
      ]
    ]
  ]
]
\end{oltableau}

\bigskip

Both of these false $\Box$ sentences have to be made false somehow.

## $\Box(\Box A \rightarrow B) \vee \Box(\Box B \rightarrow A)$

\begin{oltableau}
[\pFmla{\False}{\Box(\Box A \rightarrow B) \vee \Box(\Box B \rightarrow A)}{1}, just = \TAss,
  [\pFmla{\False}{\Box(\Box A \rightarrow B)}{1}, just = {\TRule{\False}{\vee}[1]}
    [\pFmla{\False}{\Box(\Box B \rightarrow A)}{1}, just = {\TRule{\False}{\vee}[1]}
      [\pFmla{\False}{\Box A \rightarrow B}{2}, just = {\TRule{\False}{\Box}[2]}
        [\pFmla{\False}{\Box B \rightarrow A}{3}, just = {\TRule{\False}{\Box}[3]}
          [\pFmla{\True}{\Box A}{2}, just = {\TRule{\False}{\rightarrow}[4]}
            [\pFmla{\False}{B}{2}, just = {\TRule{\False}{\rightarrow}[4]}
              [\pFmla{\True}{\Box B}{3}, just = {\TRule{\False}{\rightarrow}[5]}
                [\pFmla{\False}{A}{3}, just = {\TRule{\False}{\rightarrow}[5]}
                ]
              ]
            ]
          ]
        ]
      ]
    ]
  ]
]
\end{oltableau}

\bigskip

- False $\rightarrow$ sentences mean left false; right true.


## $\Box(\Box A \rightarrow B) \vee \Box(\Box B \rightarrow A)$

\begin{oltableau}
[\pFmla{\False}{\Box(\Box A \rightarrow B) \vee \Box(\Box B \rightarrow A)}{1}, just = \TAss,
  [\pFmla{\False}{\Box(\Box A \rightarrow B)}{1}, just = {\TRule{\False}{\vee}[1]}
    [\pFmla{\False}{\Box(\Box B \rightarrow A)}{1}, just = {\TRule{\False}{\vee}[1]}
      [\pFmla{\False}{\Box A \rightarrow B}{1.1}, just = {\TRule{\False}{\Box}[2]}
        [\pFmla{\False}{\Box B \rightarrow A}{1.2}, just = {\TRule{\False}{\Box}[3]}
          [\pFmla{\True}{\Box A}{2}, just = {\TRule{\False}{\rightarrow}[4]}
            [\pFmla{\False}{B}{2}, just = {\TRule{\False}{\rightarrow}[4]}
              [\pFmla{\True}{\Box B}{3}, just = {\TRule{\False}{\rightarrow}[5]}
                [\pFmla{\False}{A}{3}, just = {\TRule{\False}{\rightarrow}[5]}
                  [\pFmla{\True}{A}{3}, just = {\TRule{\True}{\Box}[6]}, close]
                ]
              ]
            ]
          ]
        ]
      ]
    ]
  ]
]
\end{oltableau}

\bigskip

- And if $\Box A$ is true, then $A$ is true everywhere, including 3.
- This closes the tree, so it is a theorem of S5.


# $\Diamond A \rightarrow \Box \Diamond A$ (in S5)


## Hypothesis

$\Diamond A \rightarrow \Box \Diamond A$ is a theorem of S5.

- We are going to use simplified S5 because normal S5 is really painful for cases like this one.
- Note that if we can prove this, we'll have shown in effect that in S5, all true modal claims are necessarily true. That's the distinctive feature of S5; modality itself is never contingent.

## $\Diamond A \rightarrow \Box \Diamond A$

\begin{oltableau}
[\pFmla{\False}{\Diamond A \rightarrow \Box \Diamond A}{1}, just = \TAss,
]
\end{oltableau}

\bigskip

Start with it being false at 1.

## $\Diamond A \rightarrow \Box \Diamond A$

\begin{oltableau}
[\pFmla{\False}{\Diamond A \rightarrow \Box \Diamond A}{1}, just = \TAss,
  [\pFmla{\True}{\Diamond A}{1}, just = {\TRule{\False}{\rightarrow}[1]}
    [\pFmla{\False}{\Box \Diamond A}{1}, just = {\TRule{\False}{\rightarrow}[1]}
    ]
  ]
]
\end{oltableau}

\bigskip

This feels familiar by now.

## $\Diamond A \rightarrow \Box \Diamond A$

\begin{oltableau}
[\pFmla{\False}{\Diamond A \rightarrow \Box \Diamond A}{1}, just = \TAss,
  [\pFmla{\True}{\Diamond A}{1}, just = {\TRule{\False}{\rightarrow}[1]}
    [\pFmla{\False}{\Box \Diamond A}{1}, just = {\TRule{\False}{\rightarrow}[1]}
      [\pFmla{\True}{A}{2}, just = {\TRule{\True}{\Diamond}[2]}
        [\pFmla{\False}{\Diamond A}{3}, just = {\TRule{\False}{\Box}[3]}
        ]
      ]
    ]
  ]
]
\end{oltableau}

\bigskip

- True $\Diamond$ sentences and false $\Box$ sentences have to be made true somewhere.
- Not necessarily the same 'somewhere'.

## $\Diamond A \rightarrow \Box \Diamond A$

\begin{oltableau}
[\pFmla{\False}{\Diamond A \rightarrow \Box \Diamond A}{1}, just = \TAss,
  [\pFmla{\True}{\Diamond A}{1}, just = {\TRule{\False}{\rightarrow}[1]}
    [\pFmla{\False}{\Box \Diamond A}{1}, just = {\TRule{\False}{\rightarrow}[1]}
      [\pFmla{\True}{A}{2}, just = {\TRule{\True}{\Diamond}[2]}
        [\pFmla{\False}{\Diamond A}{3}, just = {\TRule{\False}{\Box}[3]}
          [\pFmla{\False}{A}{3}, just = {\TRule{\False}{\Diamond}[5]}]
        ]
      ]
    ]
  ]
]
\end{oltableau}

\bigskip

- False $\Diamond$ sentences are false everywhere.
- That is, the part inside the $\Diamond$ is false everywhere.

## $\Diamond A \rightarrow \Box \Diamond A$

\begin{oltableau}
[\pFmla{\False}{\Diamond A \rightarrow \Box \Diamond A}{1}, just = \TAss,
  [\pFmla{\True}{\Diamond A}{1}, just = {\TRule{\False}{\rightarrow}[1]}
    [\pFmla{\False}{\Box \Diamond A}{1}, just = {\TRule{\False}{\rightarrow}[1]}
      [\pFmla{\True}{A}{2}, just = {\TRule{\True}{\Diamond}[2]}
        [\pFmla{\False}{\Diamond A}{3}, just = {\TRule{\False}{\Box}[3]}
          [\pFmla{\False}{A}{2}, just = {\TRule{\False}{\Diamond}[5]}, close]
        ]
      ]
    ]
  ]
]
\end{oltableau}

And so it closes, so this is a theorem.

# $\Box \Diamond A \rightarrow A$ (in S5)


## Hypothesis

$\Box \Diamond A \rightarrow A$ is a theorem of S5.

- We are going to use simplified S5. \pause
- Note this 'should' fail given what we have shown.
- We know that $\Diamond A$ implies $\Box \Diamond A$.
- So if $\Box \Diamond A$ implies $A$, we'll have $\Diamond A$ implies $A$, which is absurd.


## $\Box \Diamond A \rightarrow A$

\begin{oltableau}
[\pFmla{\False}{\Box \Diamond A \rightarrow A}{1}, just = \TAss,
]
\end{oltableau}

\bigskip

Start with it being false at 1.

## $\Box \Diamond A \rightarrow A$

\begin{oltableau}
[\pFmla{\False}{\Box \Diamond A \rightarrow A}{1}, just = \TAss,
  [\pFmla{\True}{\Box \Diamond A}{1}, just = {\TRule{\False}{\rightarrow}[1]}
    [\pFmla{\False}{A}{1}, just = {\TRule{\False}{\rightarrow}[1]}
    ]
  ]
]
\end{oltableau}

\bigskip

This feels familiar by now.

## $\Box \Diamond A \rightarrow A$

\begin{oltableau}
[\pFmla{\False}{\Box \Diamond A \rightarrow A}{1}, just = \TAss,
  [\pFmla{\True}{\Box \Diamond A}{1}, just = {\TRule{\False}{\rightarrow}[1]}
    [\pFmla{\False}{A}{1}, just = {\TRule{\False}{\rightarrow}[1]}
      [\pFmla{\True}{\Diamond A}{1}, just = {\TRule{\True}{\Box}[2]}
      ]
    ]
  ]
]
\end{oltableau}

\bigskip

The unboxed part of a box sentence is true everywhere, so it is true here.

## $\Box \Diamond A \rightarrow A$

\begin{oltableau}
[\pFmla{\False}{\Box \Diamond A \rightarrow A}{1}, just = \TAss,
  [\pFmla{\True}{\Box \Diamond A}{1}, just = {\TRule{\False}{\rightarrow}[1]}
    [\pFmla{\False}{A}{1}, just = {\TRule{\False}{\rightarrow}[1]}
      [\pFmla{\True}{\Diamond A}{1}, just = {\TRule{\True}{\Box}[2]}
        [\pFmla{\True}{A}{2}, just = {\TRule{\True}{\Diamond}[4]}
        ]
      ]
    ]
  ]
]
\end{oltableau}

\bigskip

True $\Diamond$ sentences have to be made true by some world. It can't be this one, since $A$ is false here.

## $\Box \Diamond A \rightarrow A$

\begin{oltableau}
[\pFmla{\False}{\Box \Diamond A \rightarrow A}{1}, just = \TAss,
  [\pFmla{\True}{\Box \Diamond A}{1}, just = {\TRule{\False}{\rightarrow}[1]}
    [\pFmla{\False}{A}{1}, just = {\TRule{\False}{\rightarrow}[1]}
      [\pFmla{\True}{\Diamond A}{1}, just = {\TRule{\True}{\Box}[2]}
        [\pFmla{\True}{A}{2}, just = {\TRule{\True}{\Diamond}[4]}
          [\pFmla{\True}{\Diamond A}{2}, just = {\TRule{\True}{\Box}[2]}
          ]
        ]
      ]
    ]
  ]
]
\end{oltableau}

\bigskip

True $\Box$ sentences are true, unboxed, everywhere.

## $\Box \Diamond A \rightarrow A$

\begin{oltableau}
[\pFmla{\False}{\Box \Diamond A \rightarrow A}{1}, just = \TAss,
  [\pFmla{\True}{\Box \Diamond A}{1}, just = {\TRule{\False}{\rightarrow}[1]}
    [\pFmla{\False}{A}{1}, just = {\TRule{\False}{\rightarrow}[1]}
      [\pFmla{\True}{\Diamond A}{1}, just = {\TRule{\True}{\Box}[2]}
        [\pFmla{\True}{A}{2}, just = {\TRule{\True}{\Diamond}[4]}
          [\pFmla{\True}{\Diamond A}{2}, just = {\TRule{\True}{\Box}[2]}
          ]
        ]
      ]
    ]
  ]
]
\end{oltableau}

\bigskip

Now if we are following the rules mechanically we will add a new world to make $A$ true, call it world 3. And the cycle will continue.

## $\Box \Diamond A \rightarrow A$

\begin{oltableau}
[\pFmla{\False}{\Box \Diamond A \rightarrow A}{1}, just = \TAss,
  [\pFmla{\True}{\Box \Diamond A}{1}, just = {\TRule{\False}{\rightarrow}[1]}
    [\pFmla{\False}{A}{1}, just = {\TRule{\False}{\rightarrow}[1]}
      [\pFmla{\True}{\Diamond A}{1}, just = {\TRule{\True}{\Box}[2]}
        [\pFmla{\True}{A}{2}, just = {\TRule{\True}{\Diamond}[4]}
          [\pFmla{\True}{\Diamond A}{2}, just = {\TRule{\True}{\Box}[2]}
          ]
        ]
      ]
    ]
  ]
]
\end{oltableau}

\bigskip

- But if we think through what the lines are saying, we can see that we can stop here.
- Line 6 has to be made true somehow.
- But line 5 says that world 2 itself makes line 6 true.
- So there isn't anything extra to do.

## $\Box \Diamond A \rightarrow A$

So here is a description of a model where this alleged theorem fails.

- There are two worlds: $w_1$ and $w_2$.
- At $w_1$, $A$ is false.
- At $w_2$, $A$ is true.
- Because $w_2$ exists, $\Diamond A$ is true everywhere.
- So $\Box \Diamond A$ is true everywhere.
- So at $w_1$, $\Box \Diamond A$ is true and $A$ is false.
- So at $w_1$, $\Box \Diamond A \rightarrow A$ is false.

## For Next Time

Next week we'll end the course by discussing conditionals.